src/QueryAux.v
@@ -12,19 +12,43 @@ Require Import Query.
 
 Section QueryAux.
 
-  Variables S Vals : ordType.
+  Variables Name Vals : ordType.
 
-  Implicit Type query : @Query S Vals.
+  Implicit Type query : @Query Name Vals.
+  Implicit Type response : @ResponseObject Name Vals.
   
-  Fixpoint size query : nat :=
+  Fixpoint query_size query : nat :=
     match query with
-    | NestedField _ _ q' => 1 + (size q')
-    | NestedLabeledField _ _ _ q' => 1 + (size q')
-    | InlineFragment _ q' => 1 + (size q')
-    | SelectionSet q' q'' => (size q') + (size q'')
+    | NestedField _ _ q' => 1 + (query_size q')
+    | NestedLabeledField _ _ _ q' => 1 + (query_size q')
+    | InlineFragment _ q' => 1 + (query_size q')
+    | SelectionSet q' q'' => (query_size q') + (query_size q'')
     | _ => 1
     end.
 
-
   
+  Fixpoint app_response (r1 r2 : @ResponseObject Name Vals) : ResponseObject :=
+    match r1, r2 with
+    | ResponseList rs, ResponseList rs' => ResponseList (rs ++ rs')
+    | ResponseList rs, _ => ResponseList (rs ++ [:: r2])
+    | _, ResponseList rs' => ResponseList (r1 :: rs')
+    | _, _ => ResponseList [:: r1; r2]
+    end.
+
+  Program Fixpoint response_size response : {m : nat | 0 < m} :=
+    match response with
+    | Empty => 1
+    | Null _ => 3
+    | SingleResult _ _ => 3
+    | ListResult _ vals => 4 + size vals
+    | NestedResult _ r' => 4 + response_size r'
+    | NestedListResult _ rs => 4 + 2 * (size rs) + sumn (map (fun r => proj1_sig (response_size r)) rs)
+    | ResponseList rs => 1 + sumn (map (fun r => proj1_sig (response_size r)) rs)
+    end.
+
+  Check response_size.
+  Print response_size.
+
 End QueryAux.
+
+Arguments response_size [Name Vals].
