src/QuerySemantic.v
@@ -2,83 +2,244 @@ From mathcomp Require Import all_ssreflect.
 Set Implicit Arguments.
 Unset Strict Implicit.
 Unset Printing Implicit Defensive.
+Set Asymmetric Patterns.
 
 From extructures Require Import ord fmap.
+
 
 Require Import SchemaWellFormedness.
 Require Import GraphConformance.
 Require Import QueryConformance.
 Require Import SchemaAux.
 Require Import GraphAux.
+Require Import QueryAux.
 
 Require Import Schema.
 Require Import Query.
 Require Import Graph.
 
 
+Require Import CpdtTactics.
+
+Require Import Program.
+Require Import Omega.
+Require Import Extraction.
 
 Section QuerySemantic.
 
   Variables N Name Vals : ordType.
 
+  
+  (*Definition response_size_order (r1 r2 : @ResponseObject Name Vals) : Prop :=
+    response_size r1 < response_size r2.
 
-  Fixpoint eval (schema : @wfSchema Name Vals)  (g : graphQLGraph) (u : @node N Name Vals) (query : Query) : @ResponseObject Name Vals :=
-    match query with
-    | SingleField name args => match u.(fields) (Field name args) with
-                              | Some (inl value) => SingleResult name value
-                              | _ => Null name
-                              end
-    | LabeledField label name args =>  match u.(fields) (Field name args) with
-                                      | Some (inl value) => SingleResult label value
-                                      | _ => Null name
-                                      end
-    | NestedField name args ϕ => let target_nodes := get_target_nodes_with_field g u (Field name args) in
-                                match lookup_field_type schema (NamedType u.(type)) name with
-                                | Some (ListType _) =>
-                                  NestedListResult name (map (fun v => eval schema g v ϕ) target_nodes)
-                                | Some (NamedType _) =>
-                                  match ohead target_nodes with
-                                  | Some v => (NestedResult name (eval schema g v ϕ))
-                                  | _ => Null name
-                                  end
-                                | _ => Null name         (* If the field ∉ fields(u) then it's null, right? *)
-                                end
-                                    
-    | NestedLabeledField label name args ϕ =>  let target_nodes := get_target_nodes_with_field g u (Field name args) in
-                                match lookup_field_type schema (NamedType u.(type)) name with
-                                | Some (ListType _) =>
-                                  NestedListResult label (map (fun v => eval schema g v ϕ) target_nodes)
-                                | Some (NamedType _) =>
-                                  match ohead target_nodes with
-                                  | Some v => (NestedResult label (eval schema g v ϕ))
-                                  | _ => Null name
-                                  end
-                                | _ => Null name         
-                                end
-    | InlineFragment t ϕ => match lookup_type schema (NamedType t) with
-                           | Some (ObjectTypeDefinition _ _ _) => if t == u.(type) then
-                                                                   eval schema g u ϕ
-                                                                 else
-                                                                   Empty
-                           | Some (InterfaceTypeDefinition _ _) => if declares_implementation schema (NamedType u.(type)) (NamedType t) then
-                                                                    eval schema g u ϕ
-                                                                  else
-                                                                    Empty
-                           | Some (UnionTypeDefinition _ mbs) => if (NamedType u.(type)) \in mbs then
-                                                                  eval schema g u ϕ
-                                                                else
-                                                                  Empty
-                           | _ => Empty
-                           end
-    | SelectionSet ϕ ϕ' => ResponseList (eval schema g u ϕ) (eval schema g u ϕ')
+  Hint Constructors Acc.
+
+  Lemma response_size_order_wf' : forall len r, response_size r <= len -> Acc response_size_order r.
+  Proof.
+    rewrite /response_size_order; elim.
+    move=> rs; rewrite leqn0; move/eqP=> H.
+    apply Acc_intro; rewrite H => y H'; inversion H'.
+    move=> n IH r H; apply Acc_intro => y Hl.
+    apply: IH; move: (leq_trans Hl H); auto.
+  Defined.
+  
+  Theorem response_size_order_wf : well_founded response_size_order.
+  Proof.
+    red; intro; eapply response_size_order_wf'; eauto.
+  Defined.*)
+
+
+
+  Fixpoint indexed_β_filter (response : @ResponseObject Name Vals) (filter :  @ResponseObject Name Vals) (index : nat) : ResponseObject :=
+    match response, filter with
+    | NestedListResult l rs, NestedListResult l' rs' => if l == l' then
+                                                         nth Empty rs index
+                                                       else
+                                                         Empty
+    | ResponseList rs, NestedListResult _ _ => ResponseList (map (fun r => (indexed_β_filter r filter index)) rs)
+    | _, _ => Empty
+    end.
+  (*
+    Fixpoint indexed_β_filter (response : @ResponseObject Name Vals) (indexed_result : nat * @ResponseObject Name Vals) : ResponseObject :=
+    match response, indexed_result with
+    | NestedListResult l rs, (i, NestedListResult l' rs') => if l == l' then
+                                                              nth Empty rs i
+                                                            else
+                                                              Empty
+    | _, _ => Empty
+    end.
+   *)                                             
+  Fixpoint β_filter (filter_response response : @ResponseObject Name Vals) : @ResponseObject Name Vals :=
+    match response, filter_response with
+    | NestedResult l χ, NestedResult l' _ => if (l == l') then χ else Empty
+    | ResponseList rs, _ => ResponseList (map (β_filter filter_response) rs)
+    | _, _ => Empty
     end.
 
+  
+  Lemma t : forall n x, n < 1 + n + x.
+  Proof. crush. Qed.
 
-  Definition eval_query (schema : @wfSchema Name Vals)  (g : @conformedGraph N Name Vals schema) (query : @wfQuery Name Vals schema) : @ResponseObject Name Vals :=
-    let: WFQuery query _ := query in
-    eval schema g.(graph) g.(graph).(root) query.
+  
 
+  Lemma asdf : forall (n : nat) (m : {m : nat | 0 < m}),  n < `m + n.
+  Proof. move=> n m; case: m; crush. Qed.
+
+  Hint Resolve  t neq_0_lt asdf.
+  
+  Definition responses_size (responses : seq (@ResponseObject Name Vals)) : nat :=
+    sumn (map (fun r => proj1_sig (response_size r)) responses).
+
+  Open Scope coq_nat.
+
+  Obligation Tactic := crush.
+  Program Fixpoint γ_filter (filter_response : ResponseObject) (responses : seq ResponseObject) {measure (responses_size responses)} : seq (@ResponseObject Name Vals) :=
+    match responses with
+    | [::] => [::]
+    | response :: tl =>
+      let γ_filtered := γ_filter filter_response tl in
+      match response, filter_response with
+      | NestedResult l _, NestedResult l' _ => if l == l' then γ_filtered else response :: γ_filtered
+      | NestedListResult l _, NestedListResult l' _ => if l == l' then γ_filtered else response :: γ_filtered
+      | ResponseList rs, _ => (ResponseList (γ_filter filter_response rs)) :: γ_filtered
+      | _, _ => if response == filter_response then γ_filtered else response :: γ_filtered
+      end
+    end.
+  Next Obligation.
+    rewrite /responses_size /=; case (response_size response); crush.
+  Defined.
+  Next Obligation.
+    rewrite /responses_size /=; crush.
+  Defined.
+
+  
+  About γ_filter.
+  Check γ_filter.
+  Print γ_filter.
+  Notation "'ϵ'" := Empty.
+  Notation "l <- 'null'" := (Null l) (at level 50).
+  Notation "l <- v" := (SingleResult l v) (at level 50).
+  Notation "l <<- vals" := (ListResult l vals) (at level 50).
+  Notation "l <- {{ ρ }}" := (NestedResult l ρ) (at level 40). 
+  Notation "l <<- [{ ρ }]" := (NestedListResult l ρ) (at level 40).
+  Notation "[- ρ -]" := (ResponseList ρ) (at level 40).
+
+  Variables (l : Name) (v : Vals).
+  Eval compute in proj1_sig (response_size ([- [:: (l <- v)] -])).
+  
+  Eval compute in (γ_filter (l <- v) [:: (l <- v)]).
+
+  
+  Section Map.
     
-      
+    Variables (T1 T2 : Type) (x2 : T2) (f : nat -> T1 -> T2) (s : seq T1).
+    Definition indexed_map s :=
+      let fix imap (f : nat -> T1 -> T2) (s : seq T1) i {struct s} : seq T2 :=
+          if s is hd :: tl then (f i hd) :: imap f tl (i + 1) else [::]
+      in
+      imap f s 0.
+
+  End Map.
+  
+  Example sum_index : indexed_map (fun i x => x + i) [:: 1; 2; 3] = [:: 1; 3; 5].
+  Proof. by []. Qed.
+
+
+  Lemma γ_empty_preserves : forall l, γ_filter ϵ l = l.
+  Proof.
+    elim=> [| r rs IH] //=.
+    rewrite /γ_filter. 
+    elim=> [| r rs IH] //.
+    case: r => //=.
+    move=> rs' /=. rewrite /γ_filter.
+    
+    Open Scope coq_nat.
+    Program Fixpoint collect_list (responses : seq ResponseObject) {measure (size responses)}: seq ResponseObject :=
+      match responses with
+      | [::] => responses
+      | hd :: tl =>
+        let γ_filtered := (γ_filter hd) tl in
+        match hd with
+        | Empty => hd :: (collect_list γ_filtered)
+        | NestedResult l σ => (NestedResult l (ResponseList (collect_list (σ :: (map (β_filter hd) tl))))) :: (collect_list γ_filtered)
+        | NestedListResult l rs => (NestedListResult l (indexed_map (fun i r => ResponseList (map (fun r' => indexed_β_filter r' r i) tl)) rs)) :: (collect_list γ_filtered)
+        | ResponseList ρ => collect_list ρ
+        | _ => hd :: (collect_list γ_filtered)
+        end
+      end.
+    Next Obligation.
+      simpl. rewrite γ_empty_preserves. case: tl collect_list => [| r rs collect_list] //.
+        by move=> _.
+        
+        
+        Admit Obligations.
+
+        
+        Fixpoint collect (response : @ResponseObject Name Vals) : @ResponseObject Name Vals :=
+          match response with
+          | ResponseList rs => ResponseList (collect_list rs)                         
+          | _ => response
+          end.
+        
+        
+        Fixpoint eval (schema : @wfSchema Name Vals)  (g : graphQLGraph) (u : @node N Name Vals) (query : Query) : @ResponseObject Name Vals :=
+          match query with
+          | SingleField name args => match u.(fields) (Field name args) with
+                                    | Some (inl value) => SingleResult name value
+                                    | _ => Null name
+                                    end
+          | LabeledField label name args =>  match u.(fields) (Field name args) with
+                                             | Some (inl value) => SingleResult label value
+                                             | _ => Null name
+                                             end
+          | NestedField name args ϕ => let target_nodes := get_target_nodes_with_field g u (Field name args) in
+                                       match lookup_field_type schema (NamedType u.(type)) name with
+                                       | Some (ListType _) =>
+                                         NestedListResult name (map (fun v => eval schema g v ϕ) target_nodes)
+                                       | Some (NamedType _) =>
+                                         match ohead target_nodes with
+                                         | Some v => (NestedResult name (eval schema g v ϕ))
+                                         | _ => Null name
+                                         end
+                                       | _ => Null name         (* If the field ∉ fields(u) then it's null, right? *)
+                                       end
+                                         
+          | NestedLabeledField label name args ϕ =>  let target_nodes := get_target_nodes_with_field g u (Field name args) in
+                                                     match lookup_field_type schema (NamedType u.(type)) name with
+                                                     | Some (ListType _) =>
+                                                       NestedListResult label (map (fun v => eval schema g v ϕ) target_nodes)
+                                                     | Some (NamedType _) =>
+                                                       match ohead target_nodes with
+                                                       | Some v => (NestedResult label (eval schema g v ϕ))
+                                                       | _ => Null name
+                                                       end
+                                                     | _ => Null name         
+                                                     end
+          | InlineFragment t ϕ => match lookup_type schema (NamedType t) with
+                                  | Some (ObjectTypeDefinition _ _ _) => if t == u.(type) then
+                                                                           eval schema g u ϕ
+                                                                         else
+                                                                           Empty
+                                  | Some (InterfaceTypeDefinition _ _) => if declares_implementation schema (NamedType u.(type)) (NamedType t) then
+                                                                            eval schema g u ϕ
+                                                                          else
+                                                                            Empty
+                                  | Some (UnionTypeDefinition _ mbs) => if (NamedType u.(type)) \in mbs then
+                                                                          eval schema g u ϕ
+                                                                        else
+                                                                          Empty
+                                  | _ => Empty
+                                  end
+          | SelectionSet ϕ ϕ' => collect (ResponseList (eval schema g u ϕ) (eval schema g u ϕ'))
+          end.
+
+
+        Definition eval_query (schema : @wfSchema Name Vals)  (g : @conformedGraph N Name Vals schema) (query : @wfQuery Name Vals schema) : @ResponseObject Name Vals :=
+          let: WFQuery query _ := query in
+          eval schema g.(graph) g.(graph).(root) query.
+
+        
+        
 
 End QuerySemantic.
